src/PushButtonSynthesis/SaturatedSolinas.v
@@ -68,6 +68,7 @@ Section __.
           {emit_primitives : emit_primitives_opt}
           {should_split_mul : should_split_mul_opt}
           {should_split_multiret : should_split_multiret_opt}
+          {unfold_value_barrier : unfold_value_barrier_opt}
           {widen_carry : widen_carry_opt}
           (widen_bytes : widen_bytes_opt := true) (* true, because we don't allow byte-sized things anyway, so we should not expect carries to be widened to byte-size when emitting C code *)
           (s : Z)
