src/Rewriter/PerfTesting/Core.v
@@ -52,6 +52,7 @@ Local Instance : only_signed_opt := false.
 Local Instance : no_select_opt := false.
 Local Instance : should_split_mul_opt := false.
 Local Instance : should_split_multiret_opt := false.
+Local Instance : unfold_value_barrier_opt := true.
 Local Instance : widen_bytes_opt := false.
 Local Instance : widen_carry_opt := false.
 Local Instance : tight_upperbound_fraction_opt := default_tight_upperbound_fraction.
