src/Util/FueledLUB.v
@@ -1,0 +1,14 @@
+Fixpoint fueled_lub {A}
+         (Aeq : A -> A -> bool)
+         (join : A -> A -> A)
+         (fuel : nat)
+         (f : A -> A) (x : A)
+: bool (* fixpoint reached *) * A
+:= match fuel with
+   | 0 => (false, x)
+   | S n
+     => let fx := join x (f x) in
+        if Aeq x fx
+        then (true, fx)
+        else @fueled_lub A Aeq join n f fx
+   end.
